Moved ffi model to separate file, started work on proving lemma about reference irrelevance for compiled payload code (beefed up assumptions on config funcs as needed), and did a bunch of work on main correctness proof

projection/proofs/payload_to_cakemlProofScript.sml
@@ -1,19 +1,32 @@
 open preamble
      endpoint_to_payloadTheory (* for compile_message only*)
      payloadLangTheory payload_to_cakemlTheory
-     evaluateTheory terminationTheory ml_translatorTheory evaluatePropsTheory
+     evaluateTheory terminationTheory ml_translatorTheory ml_progTheory evaluatePropsTheory
      semanticPrimitivesTheory
      ffiTheory
+     comms_ffiTheory
      payloadPropsTheory
-     payloadSemanticsTheory
-     astBakeryTheory;
+     payloadSemanticsTheory;
 
 val _ = new_theory "payload_to_cakemlProof";
+
+val pres_ref_def = Define
+  ‘
+  pres_ref cl =
+     ∀v.
+      ∃env exp mc dc refs' u.
+        do_opapp [cl; v] = SOME (env,exp) ∧
+        (∀sc :comms_state semanticPrimitives$state.
+          (mc ≤ sc.clock ⇔ (evaluate sc env [exp] = (sc with <| clock := sc.clock - dc; refs := sc.refs ++ refs' |>, Rval [u]))) ∧
+          (mc > sc.clock ⇔ ∃es. evaluate sc env [exp] = (es, Rerr (Rabort Rtimeout_error)))
+        )
+  ’;
 
 val has_v_def = Define
   ‘has_v env n cfty f =
    (∃v. nsLookup env n = SOME v
-        ∧ cfty f v)
+        ∧ cfty f v
+        ∧ pres_ref v)
   ’;
 
 val WORD8 = “WORD:word8 -> v -> bool”;
@@ -604,51 +617,6 @@ val sem_env_cor_def =
 
 (* UNDERSTANDING WHAT LABELS MEAN IN CAKEML LAND - CONSISTENCY OF STATE *)
 
-(* MODEL OF OUTSIDE WORLD (FFI)*)
-val _ = type_abbrev("message" , “: proc # datum”);
-
-val _ = Datatype‘
-  comms_state = <| sent_messages    : message list ;
-                   receive_messages : message llist
-                 |>
-’;
-
-val ffi_send_def =
-    Define
-    ‘
-        ffi_send net_state dest data =
-            Oracle_return (net_state with sent_messages updated_by (CONS (dest,data))) data
-    ’;
-
-val find_first_def =
-    Define
-    ‘
-    find_first P ll =
-        case $OLEAST (λn. ∃x. (LNTH n ll = SOME x) ∧ P x) of
-                SOME n => SOME (THE (LTAKE n ll), THE (LNTH n ll), THE (LDROP (SUC n) ll))
-            |   NONE   => NONE
-    ’;
-
-val ffi_receive_def =
-    Define
-    ‘
-        ffi_receive net_state src _ =
-            case find_first (λ(p,_). p = src) net_state.receive_messages of
-                    SOME (q1,(p,d),q2)  => Oracle_return (net_state with receive_messages := LAPPEND (fromList q1) q2) d
-                |   NONE                => Oracle_final FFI_diverged
-    ’;
-
-val comms_ffi_oracle_def = Define
-‘
-  comms_ffi_oracle name =
-    if name = "send" then
-        ffi_send
-    else if name = "receive" then
-        ffi_receive
-    else
-        (λ _ _ _. Oracle_final FFI_failed)
-’;
-
 (* CHECK OF FFI STATE AND PAYLOAD STATE CONSISTENCY WITH LABELS *)
 val check_ffi_past_def =
     Define
@@ -656,21 +624,29 @@ val check_ffi_past_def =
     check_ffi_past pySt ffiSt = (LTAKE (LENGTH pySt.queue) ffiSt.receive_messages = SOME pySt.queue)
     ’;
 
+val get_ffi_future_def =
+    Define
+    ‘
+    get_ffi_future pySt ffiSt = case (LDROP (LENGTH pySt.queue) ffiSt.receive_messages) of
+                                        SOME x => x
+                                    |   NONE   => LNIL
+    ’;
+
 val ffi_stat_prog_cons_def =
     Define
     ‘
     ffi_stat_prog_cons pySt1 ffiSt1 lab pySt2 ffiSt2 =
-        let
-            get_fut =  (λpySt ffiSt.
-                            LDROP (LENGTH pySt.queue) ffiSt.receive_messages)
-        in
-            (check_ffi_past pySt1 ffiSt1) ∧
-            (check_ffi_past pySt2 ffiSt2) ∧
-            (get_fut pySt1 ffiSt1 = get_fut pySt2 ffiSt2) ∧
-            (case lab of
-                    LSend _ data dest   => (ffiSt2.sent_messages = (dest,data)::ffiSt1.sent_messages)
-                |   _                   => (ffiSt2.sent_messages = ffiSt1.sent_messages)
-            )
+        ((check_ffi_past pySt1 ffiSt1) ∧
+        (check_ffi_past pySt2 ffiSt2) ∧
+        (case lab of
+                LReceive src data _ => (get_ffi_future pySt1 ffiSt1 = (src,data):::get_ffi_future pySt2 ffiSt2)
+            |   _                   => (get_ffi_future pySt1 ffiSt1 = get_ffi_future pySt2 ffiSt2)
+        ) ∧
+        (case lab of
+                LSend _ data dest   => (ffiSt2.sent_messages = (dest,data)::ffiSt1.sent_messages)
+            |   _                   => (ffiSt2.sent_messages = ffiSt1.sent_messages)
+        )
+        )
     ’;
 
 val stat_prog_cor_def =
@@ -682,27 +658,283 @@ val stat_prog_cor_def =
         (ckSt2.ffi.oracle = comms_ffi_oracle))
     ’;
 
+Theorem payload_cakeml_proj_irrelrefs:
+  ∀sc0 se conf vs ep sc1 res.
+    env_asm se conf ∧
+    evaluate sc0  se  [compile_endpoint conf vs ep]  = (sc1, res)
+    ⇒
+    ∃δ. sc1.refs = sc0.refs ++ δ ∧
+        ∀refs'. evaluate (sc0 with refs := refs') se [compile_endpoint conf vs  ep] =
+                (sc1 with refs := refs' ++ δ, res)
+Proof
+  Induct_on ‘ep’
+  (* Nil endpoint case *)
+  >- (rw[compile_endpoint_def,evaluate_def] >>
+      fs[build_conv_def,do_con_check_def])
+  (* Send endpoint case *)
+  >- (simp[compile_endpoint_def,evaluate_def] >>
+      rw[AllCaseEqs ()] >>
+      fs[PULL_EXISTS] >>
+      rename [‘evaluate _ lenv [lexp] = (_,_)’,
+                  ‘nsLookup _ (Short mlistNm) = SOME mval’,
+                  ‘nsLookup _ conf.length = SOME lc’]
+      >- (drule_then assume_tac (CONJUNCT1 evaluate_length) >>
+          fs[] >>
+          rename [‘evaluate _ lenv [lexp] = (_,Rval lvs)’] >>
+          ‘∃lv. lvs = [lv]’
+            by (Cases_on ‘lvs’ >> fs[]) >>
+          rw[] >> fs[] >>
+          ‘pres_ref lc’
+            by fs[env_asm_def,has_v_def] >>
+          fs[pres_ref_def] >>
+          cheat
+          (*
+          pop_assum (qspec_then ‘mval’ (qx_choose_then ‘δ’ assume_tac)) >>
+          qexists_tac ‘δ’ >>
+          rfs[] >>
+          fs[eval_rel_def] >>
+          cheat
+          *)
+          )
+      >- (cheat)
+      >- (cheat)
+      >- (cheat)
+      >- (cheat))
+(*          >> 
+        )
+      Cases_on ‘nsLookup se.v (Short s)’ >>
+      fs[] >>
+      Cases_on ‘nsLookup se.v conf.length’ >>
+      fs[] >>
+      Cases_on ‘res’ >>
+      fs[] >>
+      qexists_tac ‘refs'’ >>
+      simp[] >>
+      Cases_on ‘do_opapp [x'; x]’
+      >- fs[]
+      >- (fs[]
 
 
-Theorem payload_cakeml_projection
-    ‘
+      >- (fs[] >>
+          Cases_on ‘res’ >>
+          fs[] >>
+          qexists_tac ‘refs'’ >>
+          simp[])
+      >- (fs[] >>
+          Cases_on ‘nsLookup se.v conf.length’ >>
+          fs[] >>)
+
+
+      fs[]
+      Cases_on ‘’ *)
+  >- (cheat)
+  >- (cheat)
+  >- (cheat)
+QED
+
+
+Theorem payload_cakeml_proj_correct:
     ∀conf p sp sp' ep ep' L.
         trans conf (NEndpoint p sp ep) L (NEndpoint p sp' ep')
-        ⇒  (∀se vs se' vs'. ∃minClock. ∀sc sc'.
-                    (enc_ok conf se  (letfuns ep)  vs)  ∧
-                    (enc_ok conf se' (letfuns ep') vs') ∧
-                    (sem_env_cor conf sp  se)  ∧
-                    (sem_env_cor conf sp' se') ∧
-                    (stat_prog_cor sp sc L sp' sc') ∧
-                    (minClock ≤ sc.clock) ∧
-                    (minClock ≤ sc'.clock)
-                    ⇒  (∃s s' res.
-                            (evaluate sc se [compile_endpoint conf vs  ep]  = (s, res)) ∧
-                            (evaluate sc se [compile_endpoint conf vs' ep'] = (s',res)) ∧
-                            (s.ffi.ffi_state = s'.ffi.ffi_state) 
-                        )
+        ⇒  (∀se vs se' vs' sc sc'.
+                (enc_ok conf se  (letfuns ep)  vs)  ∧
+                (enc_ok conf se' (letfuns ep') vs') ∧
+                (sem_env_cor conf sp  se)  ∧
+                (sem_env_cor conf sp' se') ∧
+                (stat_prog_cor sp sc L sp' sc')
+                ⇒ ∃mc s s' res.
+                    (evaluate (sc  with clock := mc)  se  [compile_endpoint conf vs  ep]  = (s, res)) ∧
+                    (evaluate (sc' with clock := mc)  se' [compile_endpoint conf vs' ep'] = (s',res)) ∧
+                    (s.ffi.ffi_state = s'.ffi.ffi_state) 
             )
-    ’
-   (cheat);
+Proof
+    Cases_on ‘ep’
+    (* Nil Endpoint Case *)
+    >- (rpt strip_tac >>
+        Cases_on ‘L’ >>
+        fs[Once trans_cases] >>
+        (* Only LReceive Possible *)
+        rw[compile_endpoint_def,evaluate_def] >>
+        rw[do_con_check_def,build_conv_def] >>
+        (* We don't actually need all the assumptions *)
+        fs[stat_prog_cor_def,ffi_stat_prog_cons_def] >>
+        (* Everything else is equal in the record by assumptions *)
+        ‘sc.ffi.ffi_state.receive_messages = sc'.ffi.ffi_state.receive_messages’
+            suffices_by rw[comms_state_component_equality] >>
+        (* Essentially split the lists and abbreviate to allow for proof *)
+        rw[LNTH_EQ] >>
+        fs[check_ffi_past_def] >>
+        qabbrev_tac ‘LQ = LENGTH sp.queue’ >>
+        qabbrev_tac ‘OR = sc.ffi.ffi_state.receive_messages’ >>
+        qabbrev_tac ‘NR = sc'.ffi.ffi_state.receive_messages’ >>
+        ‘OR = LAPPEND (fromList (THE (LTAKE LQ OR))) (THE (LDROP LQ OR))’
+            by (‘¬LFINITE OR ∨ LQ ≤ (THE (LLENGTH OR))’
+                    by (CCONTR_TAC >>
+                        Cases_on ‘LLENGTH OR’ >>
+                        fs[LTAKE_LLENGTH_NONE] >>
+                        fs[LLENGTH]) >>
+                metis_tac[LTAKE_DROP]) >>
+        ‘NR = LAPPEND (fromList (THE (LTAKE LQ NR))) (THE (LDROP LQ NR))’
+            by (‘¬LFINITE NR ∨ LQ ≤ (THE (LLENGTH NR))’
+                    by (CCONTR_TAC >>
+                        Cases_on ‘LLENGTH NR’ >>
+                        fs[LTAKE_LLENGTH_NONE] >>
+                        fs[LLENGTH]) >>
+                metis_tac[LTAKE_DROP]) >>
+        first_x_assum (SUBST1_TAC) >>
+        first_x_assum (SUBST1_TAC) >>
+        (* Can quickly reduce to the tail equality *)
+        ‘LTAKE LQ NR = SOME sp.queue’
+            by (CCONTR_TAC >>
+                Cases_on ‘LTAKE LQ NR’ >>
+                Cases_on ‘LNTH LQ NR’ >>
+                fs[LTAKE_SNOC_LNTH]) >>
+        rw[LNTH_LAPPEND] >>
+        ‘LDROP LQ OR = LDROP LQ NR’
+            suffices_by rw[] >>
+        (* We can now squeeze out an assumption to get the info we need *)
+        fs[get_ffi_future_def] >>
+        Cases_on ‘LDROP LQ OR’ >>
+        fs[] >>
+        Cases_on ‘LDROP (SUC LQ) NR’
+        >- (fs[LDROP_SUC]
+            >- (‘LFINITE NR’
+                    by metis_tac[LDROP_NONE_LFINITE] >>
+                (* We can prove this case nonsensical based on the known info on LTAKE (SUC LQ) NR *)
+                ‘LQ = THE (LLENGTH NR)’
+                    suffices_by (rpt strip_tac >>
+                                ‘∃y. LDROP LQ NR = SOME y’
+                                    by rw[LFINITE_DROP] >>
+                                fs[]) >>
+                ‘THE (LLENGTH NR) ≤ LQ’
+                    by (CCONTR_TAC >>
+                        ‘∃y. LDROP LQ NR = SOME y’
+                            by rw[LFINITE_DROP] >>
+                        fs[]) >>
+                ‘LQ ≤ THE (LLENGTH NR)’
+                    by (CCONTR_TAC >>
+                        ‘∃l. LLENGTH NR = SOME l’
+                            by fs[LFINITE_LLENGTH] >>
+                        ‘l' < SUC LQ’
+                            by fs[THE_DEF] >>
+                        ‘LTAKE (SUC LQ) NR = NONE’
+                            by metis_tac[LTAKE_LLENGTH_NONE] >>
+                        fs[]) >>
+                simp[])
+            >- (‘LLENGTH NR = SOME LQ’
+                    by metis_tac[LDROP_EQ_LNIL] >>
+                ‘LQ < SUC LQ’
+                    by rw[] >>
+                ‘LTAKE (SUC LQ) NR = NONE’
+                    by metis_tac[LTAKE_LLENGTH_NONE] >>
+                fs[])
+            )
+        >- (fs[LDROP_SUC] >>
+            Cases_on ‘x''’
+            >> fs[LTL]
+            >> ‘SOME h = LNTH LQ NR’
+                    by rw[LNTH_HD_LDROP]
+            >> ‘LNTH LQ NR = SOME (EL LQ (SNOC (l,l0) sp.queue))’
+                    by (‘LQ < SUC LQ’
+                            by rw[] >>
+                        metis_tac[LTAKE_LNTH_EL])
+            >> ‘(l,l0) = EL LQ (SNOC (l,l0) sp.queue)’
+                    suffices_by fs[]
+            >> qunabbrev_tac ‘LQ’
+            >> rw[EL_LENGTH_SNOC])
+        )
+    (* The Send endpoint case *)
+    >- (Cases_on ‘L’ >>
+        simp[Once trans_cases]
+        (* Send Label Case *)
+        >- (rw[compile_endpoint_def]
+            (* Final Message Case *)
+            >- ((* This is just essentially translating CakeML AST back into HOL! *)
+                fs[sem_env_cor_def] >>
+                ‘∃ dc. nsLookup se.v (Short s) = SOME dc ∧ LIST_TYPE WORD d dc’
+                    by metis_tac[] >>
+                ‘has_v se.v conf.length (LIST_TYPE ^WORD8 --> NUM) LENGTH’
+                    by metis_tac[env_asm_def] >>
+                fs[has_v_def] >>
+                rename [‘(_ --> _) LENGTH lengthc’] >>
+                fs[Arrow_def, AppReturns_def] >>
+                cheat)
+                (*
+                pop_assum (drule_then assume_tac) >>
+                rw[evaluate_def] >>
+                ‘∃env exp. do_opapp [lengthc;dc] = SOME (env,exp)’
+                    by metis_tac[] >>
+                ‘∃u. NUM (LENGTH d) u’
+                    by metis_tac[] >>
+                ‘∀st :comms_state semanticPrimitives$state.
+                    ∃refs'. eval_rel st env exp (st with refs := st.refs ++ refs') u’
+                    by (‘∀refs.
+                             ∃refs'.
+                                 eval_rel (empty_state with refs := refs) env exp
+                                   (empty_state with refs := refs ++ refs') u’
+                            by (‘∀ a u1 u2. NUM a u1 ∧ NUM a u2 ⇒ (u1 = u2)’
+                                    by rw[NUM_def,INT_def] >>
+                                rpt strip_tac >>
+                                first_x_assum (qspec_then ‘refs’ assume_tac) >>
+                                fs[] >>
+                                ‘SOME (env,exp) = SOME (env',exp')’
+                                    by metis_tac[EQ_SYM_EQ] >>
+                                ‘env = env'’
+                                    by rw[] >>
+                                ‘exp = exp'’
+                                    by rw[] >>
+                                rw[] >>
+                                metis_tac[]) >>
+                        strip_tac >>
+                        pop_assum (qspec_then ‘st.refs’ assume_tac) >>
+                        fs[] >>
+                        qexists_tac ‘refs'’ >>
+                        irule evaluate_empty_state_IMP >>
+                        simp[]) >>
+                qpat_x_assum ‘∀r. ∃a b c d. P’ kall_tac >>
+                simp[] >>
+                Q.REFINE_EXISTS_TAC ‘SUC mc’ >>
+                simp[] >>
+                simp[dec_clock_def] >>
+                fs[eval_rel_def] >>
+                pop_assum (qspec_then ‘sc’ strip_assume_tac) >>
+                Q.REFINE_EXISTS_TAC ‘mc + ck1’ >>
+                ‘∀mc.
+                  (evaluate (sc with clock := mc + ck1) env [exp] =
+                    (sc with <|clock := mc + ck2; refs := sc.refs ++ refs'|>, Rval [u]))’
+                  by (strip_tac >>
+                      qabbrev_tac ‘es = (sc with clock := ck1)’ >>
+                      qabbrev_tac ‘es' = sc with <|clock := ck2; refs := sc.refs ++ refs'|>’ >>
+                      ‘evaluate (es with clock := es.clock + mc) env [exp]
+                        = (es' with clock := es'.clock + mc,Rval [u])’
+                        suffices_by  rw[Abbr ‘es’, Abbr ‘es'’] >>
+                      ‘evaluate es env [exp] = (es', Rval [u])’
+                        suffices_by rw[evaluate_add_to_clock] >>
+                      simp[]) >>
+                rw[] >>
+                simp[do_app_def] >>
+                fs[NUM_def,INT_def] >>
+                rw[opb_lookup_def] >>
+                rw[do_if_def]
+                *)
+                (* Case where LENGTH d <= n *)
+                (*
+                >- (fs[letfuns_def] >>
+                *)
+                    (* Need ref independence *)
+                    (* Need constancy of compile semantics under relation of vs to vs' *)
+                (*
+                    cheat)
+                *)
+            (* Intermediate Message Case *)
+            >- (cheat)
+          )     
+        (* Receive Label Case *)
+        >- (cheat)
+      )
+    >- (cheat)
+    >- (cheat)
+    >- (cheat)
+QED
 
 val _ = export_theory ();
