projection/proofs/comms_ffiScript.sml
@@ -1,0 +1,53 @@
+open    HolKernel
+        Parse
+        bossLib
+        astBakeryTheory
+        ffiTheory;
+
+val _ = new_theory "comms_ffi";
+
+val _ = type_abbrev("message" , “: proc # datum”);
+
+val _ = Datatype‘
+  comms_state = <| sent_messages    : message list ;
+                   receive_messages : message llist
+                 |>
+’;
+
+val ffi_send_def =
+    Define
+    ‘
+        ffi_send net_state dest data =
+            Oracle_return (net_state with sent_messages updated_by (CONS (dest,data))) data
+    ’;
+
+val find_first_def =
+    Define
+    ‘
+    find_first P ll =
+        case $OLEAST (λn. ∃x. (LNTH n ll = SOME x) ∧ P x) of
+                SOME n => SOME (THE (LTAKE n ll), THE (LNTH n ll), THE (LDROP (SUC n) ll))
+            |   NONE   => NONE
+    ’;
+
+val ffi_receive_def =
+    Define
+    ‘
+        ffi_receive net_state src _ =
+            case find_first (λ(p,_). p = src) net_state.receive_messages of
+                    SOME (q1,(p,d),q2)  => Oracle_return (net_state with receive_messages := LAPPEND (fromList q1) q2) d
+                |   NONE                => Oracle_final FFI_diverged
+    ’;
+
+val comms_ffi_oracle_def = Define
+‘
+  comms_ffi_oracle name =
+    if name = "send" then
+        ffi_send
+    else if name = "receive" then
+        ffi_receive
+    else
+        (λ _ _ _. Oracle_final FFI_failed)
+’;
+
+val _ = export_theory ();
